concurrency/juicy/semax_conc.v
@@ -12,7 +12,7 @@ Require Import VST.veric.semax.
 Require Import VST.veric.semax_call.
 Require Import VST.veric.semax_ext.
 Require Import VST.veric.juicy_safety.
-Require Import VST.veric.Clight_new.
+Require Import VST.veric.Clight_core.
 Require Import VST.veric.res_predicates.
 Require Import VST.veric.SeparationLogic.
 Require Import VST.sepcomp.extspec.
@@ -23,25 +23,25 @@ Require Import VST.floyd.client_lemmas.
 Require Import VST.floyd.jmeq_lemmas.
 Require Import VST.concurrency.common.lksize.
 Require Import VST.concurrency.juicy.semax_conc_pred.
+Require Import VST.concurrency.conclib.
 Import Clightdefs.
 Import String.
 
-Set Bullet Behavior "Strict Subproofs".
-
-(* Variables to be instantiated once the program is known. *)
+(*(* Variables to be instantiated once the program is known. *)
 Definition _f := 1%positive.      (* alpha-convertible *)
 Definition _args := 2%positive.   (* alpha-convertible *)
 Definition _lock := 1%positive.   (* alpha-convertible *)
 Definition _cond := 2%positive.   (* alpha-convertible *)
 (*Definition _lock_t := 2%positive. (* 2 (* or sometimes 3 -WM *) is the number given by
 clightgen when threads.h is included first *)*)
+*)
 
 Definition voidstar_funtype := Tfunction (Tcons (tptr tvoid) Tnil) (tptr tvoid) cc_default.
 (* Definition tlock := Tstruct _lock_t noattr. *)
-Definition tlock := (Tarray (Tpointer Tvoid noattr) 2 noattr).
+Definition tlock := (Tarray (Tpointer Ctypes.Tvoid noattr) 2 noattr).
 (* Notation tlock := tuint (only parsing). *)
 
-Goal forall (cenv: composite_env), @sizeof cenv tlock = LKSIZE.
+Goal forall (cenv: compspecs), @sizeof cenv tlock = LKSIZE.
 Proof. reflexivity. Qed.
 
 Definition selflock_fun Q sh p : (unit -> mpred) -> (unit -> mpred) :=
@@ -50,14 +50,6 @@ Definition selflock_fun Q sh p : (unit -> mpred) -> (unit -> mpred) :=
 Definition selflock' Q sh p : unit -> mpred := HORec (selflock_fun Q sh p).
 Definition selflock Q sh p : mpred := selflock' Q sh p tt.
 
-Lemma nonexpansive_entail (F: pred rmap -> pred rmap) : nonexpansive F -> forall P Q, (P <=> Q |-- F P <=> F Q)%logic.
-Proof.
-  intros N P Q.
-  specialize (N P Q).
-  eapply derives_trans; [ eapply derives_trans | ]; [ | apply N | ];
-  apply derives_refl.
-Qed.
-
 Lemma HOnonexpansive_nonexpansive: forall F: mpred -> mpred, nonexpansive F <-> HOnonexpansive (fun P (_ : unit) => F (P tt)).
 Proof.
   intros.
@@ -65,36 +57,25 @@ Proof.
   + intros P Q.
     specialize (H (P tt) (Q tt)).
     rewrite !allp_unit.
-    auto.
+    constructor; auto.
   + intros P Q.
     specialize (H (fun x => P) (fun x => Q)).
     rewrite !allp_unit in H.
-    auto.
+    destruct H; auto.
 Qed.
 
 Lemma selflock'_eq Q sh p : selflock' Q sh p =
   selflock_fun Q sh p (selflock' Q sh p).
 Proof.
-  apply HORec_fold_unfold, prove_HOcontractive.
+  apply HORec_fold_unfold, prove_HOcontractive'.
   intros P1 P2 u.
   apply subp_sepcon; [ apply subp_refl | ].
-  rewrite <- subp_later.
-  repeat intro.
-  match goal with |- app_pred (?P >=> ?Q)%logic ?a => change (subtypes.fash (P --> Q) a) end.
-  unfold lock_inv; repeat intro.
-  destruct H3 as (b & ofs & ? & Hl & ?); exists b, ofs; split; auto; split; auto.
-  intro l; specialize (Hl l); simpl in *.
-  if_tac; auto.
-  destruct Hl as [rsh Hl]; exists rsh; rewrite Hl; repeat f_equal.
-  extensionality.
-  specialize (H tt); rewrite <- eqp_later in H.
-  specialize (H _ H0).
-  apply necR_level in H2.
-  apply predicates_hered.pred_ext; intros ? []; split; auto.
-  - destruct (H a0) as [X _]; [omega|].
-    specialize (X _ (necR_refl _)); auto.
-  - destruct (H a0) as [_ X]; [omega|].
-    specialize (X _ (necR_refl _)); auto.
+  apply allp_left with tt.
+  eapply derives_trans, subp_later1.
+  apply later_derives.
+  constructor.
+  eapply predicates_hered.derives_trans, eqp_subp.
+  apply nonexpansive_lock_inv.
 Qed.
 
 Lemma selflock_eq Q sh p : selflock Q sh p = (Q * |>lock_inv sh p (selflock Q sh p))%logic.
@@ -130,19 +111,19 @@ Proof.
     apply subp_sepcon; try apply subp_refl.
     apply allp_left with false.
     eapply derives_trans.
-      apply nonexpansive_entail, nonexpansive_lock_inv.
+      apply semax_conc.nonexpansive_entail, nonexpansive_lock_inv.
       apply fash_derives, andp_left1, derives_refl.
 
     (* join resource invariant *)
     repeat apply subp_sepcon; try apply subp_refl.
       apply allp_left with true.
       eapply derives_trans.
-        apply nonexpansive_entail, nonexpansive_lock_inv.
+        apply semax_conc.nonexpansive_entail, nonexpansive_lock_inv.
         apply fash_derives, andp_left1, derives_refl.
 
       apply allp_left with false.
       eapply derives_trans.
-        apply nonexpansive_entail, nonexpansive_lock_inv.
+        apply semax_conc.nonexpansive_entail, nonexpansive_lock_inv.
         apply fash_derives, andp_left1, derives_refl.
 Qed.
 
@@ -167,56 +148,7 @@ Proof.
   reflexivity.
 Qed.
 
-(* Condition variables *)
-(*Definition _cond_t := 4%positive.*)
-Definition tcond := tint.
-
-(* Does this need to be anything special? *)
-Definition cond_var {cs} sh v := @data_at_ cs sh tcond v.
-
 (*+ Specification of each concurrent primitive *)
-
-Lemma approx_eq_i':
-  forall (P Q : pred rmap) n,
-  (|> (P <=> Q))%pred n -> approx n P = approx n Q.
-Proof.
-  intros.
-apply pred_ext'; extensionality m'.
-unfold approx.
-apply and_ext'; auto; intros.
-specialize (H (level m')); spec H; [simpl; apply later_nat; auto |].
-specialize (H m').
-spec H; [omega |].
-destruct H.
-specialize (H m').
-specialize (H1 m').
-apply prop_ext; split; auto.
-Qed.
-
-Lemma fash_equiv_approx: forall n (R: pred rmap),
-  (|> (R <=> approx n R))%pred n.
-Proof.
-  intros.
-  intros m ? x ?; split; intros y ? ?.
-  + apply approx_lt; auto.
-    apply necR_level in H1.
-    apply later_nat in H; omega.
-  + eapply approx_p; eauto.
-Qed.
-
-Lemma nonexpansive_super_non_expansive: forall (F: mpred -> mpred),
-  nonexpansive F ->
-  forall R n,
-  approx n (F R) = approx n (F (approx n R)).
-Proof.
-  intros.
-  apply approx_eq_i'.
-  intros m ?.
-  pose proof nonexpansive_entail _ H R (approx n R) m.
-  apply H1.
-  clear - H0.
-  apply (fash_equiv_approx n R m); auto.
-Qed.
 
 Lemma nonexpansive2_super_non_expansive: forall (F: mpred -> mpred -> mpred),
   (forall P, nonexpansive (fun Q => F P Q)) ->
@@ -225,12 +157,12 @@ Lemma nonexpansive2_super_non_expansive: forall (F: mpred -> mpred -> mpred),
   approx n (F P Q) = approx n (F (approx n P) (approx n Q)).
 Proof.
   intros.
-  apply approx_eq_i'.
+  apply semax_conc.approx_eq_i'.
   intros m ?.
-  pose proof nonexpansive_entail _ (H P) Q (approx n Q) m; cbv beta in H2.
-  spec H2; [apply (fash_equiv_approx n Q m); auto |].
-  pose proof nonexpansive_entail _ (H0 (approx n Q)) P (approx n P) m; cbv beta in H3.
-  spec H3; [apply (fash_equiv_approx n P m); auto |].
+  pose proof semax_conc.nonexpansive_entail _ (H P) Q (approx n Q) as H2; cbv beta in H2.
+  destruct H2 as [H2]; specialize (H2 m). spec H2; [apply (semax_conc.fash_equiv_approx n Q m); auto |].
+  pose proof semax_conc.nonexpansive_entail _ (H0 (approx n Q)) P (approx n P) as H3; cbv beta in H3.
+  destruct H3 as [H3]; specialize (H3 m). spec H3; [apply (semax_conc.fash_equiv_approx n P m); auto |].
   remember (F P Q) as X1.
   remember (F P (approx n Q)) as X2.
   remember (F (approx n P) (approx n Q)) as X3.
@@ -253,46 +185,38 @@ Lemma nonexpansive_2super_non_expansive: forall {A B: Type} (F: (A -> B -> mpred
 *)
 Definition acquire_arg_type: rmaps.TypeTree := rmaps.ProdType (rmaps.ConstType (val * share)) rmaps.Mpred.
 
-Definition acquire_pre: val * share * mpred -> environ -> mpred :=
-  fun args =>
-  match args with
-  | (v, sh, R) =>
+Program Definition acquire_spec :=
+  TYPE acquire_arg_type WITH v : _, sh : _, R : _
+  PRE [ tptr tvoid ]
      PROP (readable_share sh)
-     LOCAL (temp _lock v)
+     PARAMS (v)
      SEP (lock_inv sh v R)
-  end.
-
-Notation acquire_post :=
-  (fun args =>
-  match args with
-  | (v, sh, R) =>
+  POST [ tvoid ]
      PROP ()
      LOCAL ()
-     SEP (lock_inv sh v R; R)
-  end).
-
-Lemma NP_acquire_pre: @super_non_expansive acquire_arg_type (fun _ => acquire_pre).
+     SEP (lock_inv sh v R; R).
+Next Obligation.
 Proof.
   hnf.
   intros.
   destruct x as [[v sh] R]; simpl in *.
-  apply (nonexpansive_super_non_expansive
-   (fun R => (PROP (readable_share sh)  LOCAL (temp _lock v)  SEP (lock_inv sh v R)) rho)).
-  apply (PROP_LOCAL_SEP_nonexpansive
+  apply (semax_conc.nonexpansive_super_non_expansive
+   (fun R => (PROP (readable_share sh)  PARAMS (v)  SEP (lock_inv sh v R)) gargs)).
+  apply (PROP_PARAMS_GLOBALS_SEP_nonexpansive
           ((fun _ => readable_share sh) :: nil)
-          ((temp _lock v) :: nil)
+          (v :: nil)
+          nil
           ((fun R => lock_inv sh v R) :: nil));
   repeat apply Forall_cons; try apply Forall_nil.
-  + unfold compose. apply const_nonexpansive.
+  + apply const_nonexpansive.
   + apply nonexpansive_lock_inv.
 Qed.
-
-Lemma NP_acquire_post: @super_non_expansive acquire_arg_type (fun _ => acquire_post).
+Next Obligation.
 Proof.
   hnf.
   intros.
   destruct x as [[v sh] R]; simpl in *.
-  apply (nonexpansive_super_non_expansive
+  apply (semax_conc.nonexpansive_super_non_expansive
    (fun R => (PROP ()  LOCAL ()  SEP (lock_inv sh v R; R)) rho)).
   apply (PROP_LOCAL_SEP_nonexpansive
           nil
@@ -303,46 +227,29 @@ Proof.
   + apply identity_nonexpansive.
 Qed.
 
-Definition acquire_spec: funspec := mk_funspec
-  ((_lock OF tptr Tvoid)%formals :: nil, tvoid)
-  cc_default
-  acquire_arg_type
-  (fun _ => acquire_pre)
-  (fun _ => acquire_post)
-  NP_acquire_pre
-  NP_acquire_post
-.
-
 Definition release_arg_type: rmaps.TypeTree := rmaps.ProdType (rmaps.ConstType (val * share)) rmaps.Mpred.
 
-Definition release_pre: val * share * mpred -> environ -> mpred :=
-  fun args =>
-  match args with
-  | (v, sh, R) =>
+Program Definition release_spec :=
+  TYPE release_arg_type WITH v : _, sh : _, R : _
+  PRE [ tptr tvoid ]
      PROP (readable_share sh)
-     LOCAL (temp _lock v)
+     PARAMS (v)
      SEP (weak_exclusive_mpred R && emp; lock_inv sh v R; R)
-  end.
-
-Notation release_post :=
-  (fun args =>
-  match args with
-  | (v, sh, R) =>
+  POST [ tvoid ]
      PROP ()
      LOCAL ()
-     SEP (lock_inv sh v R)
-  end).
-
-Lemma NP_release_pre: @super_non_expansive release_arg_type (fun _ => release_pre).
+     SEP (lock_inv sh v R).
+Next Obligation.
 Proof.
   hnf.
   intros.
   destruct x as [[v sh] R]; simpl in *.
   apply (nonexpansive_super_non_expansive
-   (fun R => (PROP (readable_share sh)  LOCAL (temp _lock v)  SEP (weak_exclusive_mpred R && emp; lock_inv sh v R; R)) rho)).
-  apply (PROP_LOCAL_SEP_nonexpansive
+   (fun R => (PROP (readable_share sh)  PARAMS (v)  SEP (weak_exclusive_mpred R && emp; lock_inv sh v R; R)) gargs)).
+  apply (PROP_PARAMS_GLOBALS_SEP_nonexpansive
           ((fun _ => readable_share sh) :: nil)
-          ((temp _lock v) :: nil)
+          (v :: nil)
+          nil
           ((fun R => weak_exclusive_mpred R && emp)%logic :: (fun R => lock_inv sh v R) :: (fun R => R) :: nil));
   repeat apply Forall_cons; try apply Forall_nil.
   + apply const_nonexpansive.
@@ -352,8 +259,7 @@ Proof.
   + apply nonexpansive_lock_inv.
   + apply identity_nonexpansive.
 Qed.
-
-Lemma NP_release_post: @super_non_expansive release_arg_type (fun _ => release_post).
+Next Obligation.
 Proof.
   hnf.
   intros.
@@ -368,25 +274,15 @@ Proof.
   apply nonexpansive_lock_inv.
 Qed.
 
-Definition release_spec: funspec := mk_funspec
-  ((_lock OF tptr Tvoid)%formals :: nil, tvoid)
-  cc_default
-  release_arg_type
-  (fun _ => release_pre)
-  (fun _ => release_post)
-  NP_release_pre
-  NP_release_post
-.
-
 Program Definition makelock_spec cs: funspec := mk_funspec
-  ((_lock OF tptr Tvoid)%formals :: nil, tvoid)
+  (tptr tvoid :: nil, tvoid)
   cc_default
   (rmaps.ProdType (rmaps.ConstType (val * share)) rmaps.Mpred)
   (fun _ x =>
    match x with
    | (v, sh, R) =>
      PROP (writable_share sh)
-     LOCAL (temp _lock v)
+     PARAMS (v)
      SEP (@data_at_ cs sh tlock v)
    end)
   (fun _ x =>
@@ -400,13 +296,13 @@ Program Definition makelock_spec cs: funspec := mk_funspec
   _
 .
 Next Obligation.
-  intros cs; hnf.
+  hnf.
   intros.
   destruct x as [[v sh] R]; simpl in *.
   auto.
 Qed.
 Next Obligation.
-  intro cs; hnf.
+  hnf.
   intros.
   destruct x as [[v sh] R]; simpl in *.
   apply (nonexpansive_super_non_expansive
@@ -420,14 +316,14 @@ Next Obligation.
 Qed.
 
 Program Definition freelock_spec cs: funspec := mk_funspec
-  ((_lock OF tptr Tvoid)%formals :: nil, tvoid)
+  (tptr tvoid :: nil, tvoid)
   cc_default
   (rmaps.ProdType (rmaps.ConstType (val * share)) rmaps.Mpred)
   (fun _ x =>
    match x with
    | (v, sh, R) =>
      PROP (writable_share sh)
-     LOCAL (temp _lock v)
+     PARAMS (v)
      SEP (weak_exclusive_mpred R && emp; lock_inv sh v R; R)
    end)
   (fun _ x =>
@@ -441,16 +337,16 @@ Program Definition freelock_spec cs: funspec := mk_funspec
   _
 .
 Next Obligation.
-  intro cs; hnf.
+  hnf.
   intros.
   destruct x as [[v sh] R]; simpl in *.
   apply (nonexpansive_super_non_expansive
    (fun R => (PROP (writable_share sh)
-    LOCAL (temp _lock v)
-    SEP (weak_exclusive_mpred R && emp; lock_inv sh v R; R)) rho)).
-  apply (PROP_LOCAL_SEP_nonexpansive
+    PARAMS (v)
+    SEP (weak_exclusive_mpred R && emp; lock_inv sh v R; R)) gargs)).
+  apply (PROP_PARAMS_GLOBALS_SEP_nonexpansive
           ((fun _ => writable_share sh) :: nil)
-          (temp _lock v :: nil)
+          (v :: nil) nil
           ((fun R => weak_exclusive_mpred R && emp)%logic :: (fun R => lock_inv sh v R) :: (fun R => R) :: nil));
   repeat apply Forall_cons; try apply Forall_nil.
   + apply const_nonexpansive.
@@ -461,7 +357,7 @@ Next Obligation.
   + apply identity_nonexpansive.
 Qed.
 Next Obligation.
-  intro cs; hnf.
+  hnf.
   intros.
   destruct x as [[v sh] R]; simpl in *.
   apply (nonexpansive_super_non_expansive
@@ -484,14 +380,14 @@ Proof.
 Qed.
 
 Program Definition freelock2_spec cs: funspec := mk_funspec
-  ((_lock OF tptr Tvoid)%formals :: nil, tvoid)
+  (tptr tvoid :: nil, tvoid)
   cc_default
   (rmaps.ProdType (rmaps.ProdType (rmaps.ConstType (val * share * share)) rmaps.Mpred) rmaps.Mpred)
   (fun _ x =>
    match x with
    | (v, sh, sh', Q, R) =>
      PROP (writable_share sh)
-     LOCAL (temp _lock v)
+     PARAMS (v)
      SEP (weak_exclusive_mpred R && weak_rec_inv sh' v Q R && emp; lock_inv sh v R)
    end)
   (fun _ x =>
@@ -505,22 +401,22 @@ Program Definition freelock2_spec cs: funspec := mk_funspec
   _
 .
 Next Obligation.
-  intro cs; hnf.
+  hnf.
   intros.
   destruct x as [[[[v sh] sh'] Q] R]; simpl in *.
   apply (nonexpansive2_super_non_expansive
    (fun Q R => (PROP (writable_share sh)
-     LOCAL (temp _lock v)
-     SEP (weak_exclusive_mpred R && weak_rec_inv sh' v Q R && emp; lock_inv sh v R)) rho));
+     PARAMS (v)
+     SEP (weak_exclusive_mpred R && weak_rec_inv sh' v Q R && emp; lock_inv sh v R)) gargs));
   [ clear Q R; intros Q;
-    apply (PROP_LOCAL_SEP_nonexpansive
+    apply (PROP_PARAMS_GLOBALS_SEP_nonexpansive
             ((fun _ => writable_share sh) :: nil)
-            (temp _lock v :: nil)
+            (v :: nil) nil
             ((fun R => weak_exclusive_mpred R && weak_rec_inv sh' v Q R && emp)%logic :: (fun R => lock_inv sh v R) :: nil))
   | clear Q R; intros R;
-    apply (PROP_LOCAL_SEP_nonexpansive
+    apply (PROP_PARAMS_GLOBALS_SEP_nonexpansive
             ((fun _ => writable_share sh) :: nil)
-            (temp _lock v :: nil)
+            (v :: nil) nil
             ((fun Q => weak_exclusive_mpred R && weak_rec_inv sh' v Q R && emp)%logic :: (fun _ => lock_inv sh v R) :: nil))];
   repeat apply Forall_cons; try apply Forall_nil.
   + apply const_nonexpansive.
@@ -537,21 +433,21 @@ Next Obligation.
   + apply const_nonexpansive.
 Qed.
 Next Obligation.
-  intro cs; hnf.
+  hnf.
   intros.
   destruct x as [[[[v sh] sh'] Q] R]; simpl in *.
   auto.
 Qed.
 
 Program Definition release2_spec: funspec := mk_funspec
-  ((_lock OF tptr Tvoid)%formals :: nil, tvoid)
+  (tptr tvoid :: nil, tvoid)
   cc_default
   (rmaps.ProdType (rmaps.ProdType (rmaps.ConstType (val * share)) rmaps.Mpred) rmaps.Mpred)
   (fun _ x =>
    match x with
    | (v, sh, Q, R) =>
      PROP (readable_share sh)
-     LOCAL (temp _lock v)
+     PARAMS (v)
      SEP (weak_exclusive_mpred R && weak_rec_inv sh v Q R && emp; R)
    end)
   (fun _ x =>
@@ -565,22 +461,22 @@ Program Definition release2_spec: funspec := mk_funspec
   _
 .
 Next Obligation.
-  intro cs; hnf.
+  hnf.
   intros.
   destruct x as [[[v sh] Q] R]; simpl in *.
   apply (nonexpansive2_super_non_expansive
    (fun Q R => (PROP (readable_share sh)
-     LOCAL (temp _lock v)
-     SEP (weak_exclusive_mpred R && weak_rec_inv sh v Q R && emp; R)) rho));
+     PARAMS (v)
+     SEP (weak_exclusive_mpred R && weak_rec_inv sh v Q R && emp; R)) gargs));
   [ clear Q R; intros Q;
-    apply (PROP_LOCAL_SEP_nonexpansive
+    apply (PROP_PARAMS_GLOBALS_SEP_nonexpansive
             ((fun _ => readable_share sh) :: nil)
-            (temp _lock v :: nil)
+            (v :: nil) nil
             ((fun R => weak_exclusive_mpred R && weak_rec_inv sh v Q R && emp)%logic :: (fun R => R) :: nil))
   | clear Q R; intros R;
-    apply (PROP_LOCAL_SEP_nonexpansive
+    apply (PROP_PARAMS_GLOBALS_SEP_nonexpansive
             ((fun _ => readable_share sh) :: nil)
-            (temp _lock v :: nil)
+            (v :: nil) nil
             ((fun Q => weak_exclusive_mpred R && weak_rec_inv sh v Q R && emp)%logic :: (fun _ => R) :: nil))];
   repeat apply Forall_cons; try apply Forall_nil.
   + apply const_nonexpansive.
@@ -597,12 +493,13 @@ Next Obligation.
   + apply const_nonexpansive.
 Qed.
 Next Obligation.
-  intro cs; hnf.
+  hnf.
   intros.
   destruct x as [[[v sh] Q] R]; simpl in *.
   auto.
 Qed.
 
+(*
 (* condition variables *)
 Definition makecond_spec cs :=
    WITH v : val, sh : share
@@ -750,7 +647,7 @@ Definition signal_spec cs :=
      PROP ()
      LOCAL ()
      SEP (@cond_var cs shc c).
-
+*)
 
 
 (* Notes about spawn_thread:
@@ -779,7 +676,7 @@ Local Open Scope logic.
 
 (* @Qinxiang: it would be great to complete the annotation *)
 
-Definition spawn_arg_type := rmaps.ProdType (rmaps.ProdType (rmaps.ProdType (rmaps.ConstType (val * val))
+(*Definition spawn_arg_type := rmaps.ProdType (rmaps.ProdType (rmaps.ProdType (rmaps.ConstType (val * val))
   (rmaps.ArrowType (rmaps.DependentType 0) (rmaps.ConstType globals))) (rmaps.DependentType 0))
   (rmaps.ArrowType (rmaps.DependentType 0) (rmaps.ArrowType (rmaps.ConstType val) rmaps.Mpred)).
 
@@ -789,7 +686,8 @@ Definition spawn_pre :=
    match x with
    | (f, b, gv, w, pre) =>
      PROP (tc_val (tptr Tvoid) b)
-     (LOCALx (temp _f f :: temp _args b :: gvars (gv w) :: nil)
+     PARAMS (f, b)
+     GLOBALS  :: temp _args b :: gvars (gv w) :: nil
      (SEP (
        EX _y : ident,
          (func_ptr'
@@ -852,26 +750,9 @@ Definition spawn_spec := mk_funspec
   spawn_pre
   spawn_post
   spawn_pre_nonexpansive
-  spawn_post_nonexpansive.
+  spawn_post_nonexpansive.*)
 
 (*+ Adding the specifications to a void ext_spec *)
-
-(*! The void ext_spec *)
-Definition void_spec T : external_specification juicy_mem external_function T :=
-    Build_external_specification
-      juicy_mem external_function T
-      (fun ef => False)
-      (fun ef Hef ge tys vl m z => False)
-      (fun ef Hef ge ty vl m z => False)
-      (fun rv m z => False).
-
-Definition ok_void_spec (T : Type) : OracleKind.
- refine (Build_OracleKind T (Build_juicy_ext_spec _ (void_spec T) _ _ _)).
-Proof.
-  simpl; intros; contradiction.
-  simpl; intros; contradiction.
-  simpl; intros; intros ? ? ? ?; contradiction.
-Defined.
 
 Definition concurrent_simple_specs (cs : compspecs) (ext_link : string -> ident) :=
   (ext_link "acquire"%string, acquire_spec) ::
