concurrency/juicy/semax_conc_pred.v
@@ -13,7 +13,7 @@ Require Import VST.veric.semax_call.
 Require Import VST.veric.semax_ext.
 Require Import VST.veric.semax_ext_oracle.
 Require Import VST.veric.juicy_safety.
-Require Import VST.veric.Clight_new.
+Require Import VST.veric.Clight_core.
 Require Import VST.veric.res_predicates.
 Require Import VST.veric.SeparationLogic.
 Require Import VST.sepcomp.extspec.
@@ -23,69 +23,7 @@ Require Import VST.floyd.nested_field_lemmas.
 Require Import VST.floyd.client_lemmas.
 Require Import VST.floyd.jmeq_lemmas.
 Require Import VST.concurrency.common.lksize.
-
-Lemma approx_derives_ge : forall n m P, (n <= m)%nat -> approx n P |-- approx m P.
-Proof.
-  intros; change (predicates_hered.derives (approx n P) (approx m P)).
-  intros ? []; split; auto; omega.
-Qed.
-
-Lemma approx_derives : forall P n, approx n P |-- P.
-Proof.
-  exact approx_p.
-Qed.
-
-Definition exclusive_mpred (R : mpred) :=
-  (R * R |-- FF)%logic.
-
-Program Definition weak_exclusive_mpred (P: mpred): mpred :=
-  fun w => exclusive_mpred (approx (S (level w)) P).
-Next Obligation.
-  intros; hnf; intros.
-  unfold exclusive_mpred in *.
-  apply age_level in H.
-  eapply derives_trans, H0.
-  apply sepcon_derives; apply approx_derives_ge; omega.
-Defined.
-
-Lemma corable_weak_exclusive R : seplog.corable (weak_exclusive_mpred R).
-Proof.
-  change (corable.corable (weak_exclusive_mpred R)).
-  intro; simpl.
-  rewrite level_core; auto.
-Qed.
-
-Lemma exclusive_mpred_nonexpansive:
-  nonexpansive weak_exclusive_mpred.
-Proof.
-  hnf; intros.
-  intros n ?.
-  simpl in H |- *.
-  assert (forall y, (n >= level y)%nat -> (P y <-> Q y)).
-  {
-    intros; specialize (H y H0).
-    destruct H.
-    specialize (H y). spec H; [auto |].
-    specialize (H1 y). spec H1; [auto |].
-    tauto.
-  }
-  clear H.
-  intros; split; intros.
-  + unfold exclusive_mpred in *.
-    eapply derives_trans, H2.
-    match goal with |- ?P |-- ?Q => change (predicates_hered.derives P Q) end.
-    intros ? (? & ? & J & [] & []).
-    pose proof (join_level _ _ _ J) as [].
-    apply necR_level in H1.
-    do 3 eexists; eauto; split; split; try omega; apply H0; auto; omega.
-  + unfold exclusive_mpred in *.
-    eapply derives_trans, H2.
-    match goal with |- ?P |-- ?Q => change (predicates_hered.derives P Q) end.
-    intros ? (? & ? & J & [] & []).
-    pose proof (join_level _ _ _ J) as [].
-    apply necR_level in H1.
-    do 3 eexists; eauto; split; split; try omega; apply H0; auto; omega.
-Qed.
+Require Import VST.concurrency.conclib.
 
 Definition lock_inv : share -> val -> mpred -> mpred :=
   fun sh v R =>
@@ -116,134 +54,52 @@ Lemma unfash_fash_equiv: forall P Q: mpred,
   (subtypes.unfash (subtypes.fash P): mpred) <=> (subtypes.unfash (subtypes.fash Q): mpred))%pred.
 Proof.
   intros.
-  hnf; intros.
-  assert (forall y: rmap, (a >= level y)%nat -> (app_pred P y <-> app_pred Q y)).
-  {
-    intros; specialize (H y H0).
-    destruct H.
-    specialize (H y). spec H; [auto |].
-    specialize (H1 y). spec H1; [auto |].
-    tauto.
-  }
-  hnf; intros.
-  split; simpl; hnf; intros.
-  + apply necR_level in H2.
-    rewrite <- H0 by omega.
-    auto.
-  + apply necR_level in H2.
-    rewrite H0 by omega.
-    auto.
+  constructor; apply eqp_unfash.
+  rewrite eqp_nat.
+  apply predicates_hered.andp_right; eapply predicates_hered.derives_trans, subtypes.fash_K;
+    apply subtypes.fash_derives.
+  - apply predicates_hered.andp_left1; auto.
+  - apply predicates_hered.andp_left2; auto.
 Qed.
 
 Lemma iffp_equiv: forall P1 Q1 P2 Q2: mpred,
   ((P1 <=> Q1) && (P2 <=> Q2) |-- (P1 <--> P2) <=> (Q1 <--> Q2))%pred.
 Proof.
   intros.
-  hnf; intros.
-  destruct H.
-  assert (forall y: rmap, (a >= level y)%nat -> (app_pred P1 y <-> app_pred Q1 y)).
-  {
-    intros; specialize (H y H1).
-    destruct H.
-    specialize (H y). spec H; [auto |].
-    specialize (H2 y). spec H2; [auto |].
-    tauto.
-  }
-  assert (forall y: rmap, (a >= level y)%nat -> (app_pred P2 y <-> app_pred Q2 y)).
-  {
-    intros; specialize (H0 y H2).
-    destruct H0.
-    specialize (H0 y). spec H0; [auto |].
-    specialize (H3 y). spec H3; [auto |].
-    tauto.
-  }
-  split; intros; hnf; intros.
-  + split; [destruct H5 as [? _] | destruct H5 as [_ ?]]; intros ? HH; specialize (H5 _ HH).
-    - apply necR_level in H4.
-      apply necR_level in HH.
-      rewrite <- H1, <- H2 by omega.
-      auto.
-    - apply necR_level in H4.
-      apply necR_level in HH.
-      rewrite <- H1, <- H2 by omega.
-      auto.
-  + split; [destruct H5 as [? _] | destruct H5 as [_ ?]]; intros ? HH; specialize (H5 _ HH).
-    - apply necR_level in H4.
-      apply necR_level in HH.
-      rewrite H1, H2 by omega.
-      auto.
-    - apply necR_level in H4.
-      apply necR_level in HH.
-      rewrite H1, H2 by omega.
-      auto.
+  constructor; apply eqp_andp; apply subp_eqp; apply subtypes.subp_imp.
+  - apply predicates_hered.andp_left1.
+    rewrite eqp_comm; apply eqp_subp.
+  - apply predicates_hered.andp_left2.
+    apply eqp_subp.
+  - apply predicates_hered.andp_left1.
+    apply eqp_subp.
+  - apply predicates_hered.andp_left2.
+    rewrite eqp_comm; apply eqp_subp.
+  - apply predicates_hered.andp_left2.
+    rewrite eqp_comm; apply eqp_subp.
+  - apply predicates_hered.andp_left1.
+    apply eqp_subp.
+  - apply predicates_hered.andp_left2.
+    apply eqp_subp.
+  - apply predicates_hered.andp_left1.
+    rewrite eqp_comm; apply eqp_subp.
 Qed.
 
 Lemma sepcon_equiv: forall P1 Q1 P2 Q2: mpred,
   ((P1 <=> Q1) && (P2 <=> Q2) |-- (P1 * P2) <=> (Q1 * Q2))%pred.
 Proof.
   intros.
-  hnf; intros.
-  destruct H.
-  assert (forall y: rmap, (a >= level y)%nat -> (app_pred P1 y <-> app_pred Q1 y)).
-  {
-    intros; specialize (H y H1).
-    destruct H.
-    specialize (H y). spec H; [auto |].
-    specialize (H2 y). spec H2; [auto |].
-    tauto.
-  }
-  assert (forall y: rmap, (a >= level y)%nat -> (app_pred P2 y <-> app_pred Q2 y)).
-  {
-    intros; specialize (H0 y H2).
-    destruct H0.
-    specialize (H0 y). spec H0; [auto |].
-    specialize (H3 y). spec H3; [auto |].
-    tauto.
-  }
-  split; intros; hnf; intros.
-  + destruct H5 as [w1 [w2 [? [? ?]]]].
-    exists w1, w2; split; [| split]; auto.
-    - apply necR_level in H4.
-      apply join_level in H5.
-      rewrite <- H1 by omega; auto.
-    - apply necR_level in H4.
-      apply join_level in H5.
-      rewrite <- H2 by omega; auto.
-  + destruct H5 as [w1 [w2 [? [? ?]]]].
-    exists w1, w2; split; [| split]; auto.
-    - apply necR_level in H4.
-      apply join_level in H5.
-      rewrite H1 by omega; auto.
-    - apply necR_level in H4.
-      apply join_level in H5.
-      rewrite H2 by omega; auto.
+  constructor; apply eqp_sepcon.
+  - apply predicates_hered.andp_left1; auto.
+  - apply predicates_hered.andp_left2; auto.
 Qed.
 
 Lemma later_equiv: forall P Q: mpred,
   (P <=> Q |-- |> P <=> |> Q)%pred.
 Proof.
   intros.
-  hnf; intros.
-  assert (forall y: rmap, (a >= level y)%nat -> (app_pred P y <-> app_pred Q y)).
-  {
-    intros; specialize (H y H0).
-    destruct H.
-    specialize (H y). spec H; [auto |].
-    specialize (H1 y). spec H1; [auto |].
-    tauto.
-  }
-  hnf; intros.
-  split; hnf; intros; simpl in *; intros.
-  + specialize (H3 _ H4).
-    apply necR_level in H2.
-    apply laterR_level in H4.
-    rewrite <- H0 by omega.
-    auto.
-  + specialize (H3 _ H4).
-    apply necR_level in H2.
-    apply laterR_level in H4.
-    rewrite H0 by omega.
-    auto.
+  constructor; eapply predicates_hered.derives_trans, subtypes.eqp_later1.
+  apply predicates_hered.now_later.
 Qed.
 
 Lemma nonexpansive_lock_inv : forall sh p, nonexpansive (lock_inv sh p).
@@ -258,7 +114,6 @@ Proof.
   apply @const_nonexpansive.
 
   unfold LKspec.
-  apply conj_nonexpansive, const_nonexpansive.
   apply forall_nonexpansive; intros.
   hnf; intros.
   intros n ?.
@@ -267,35 +122,35 @@ Proof.
     clear - H.
     intros; specialize (H y H0).
     destruct H.
-    specialize (H y). spec H; [auto |].
-    specialize (H1 y). spec H1; [auto |].
-    tauto.
+    split; [eapply H | eapply H1]; eauto.
   }
   simpl; split; intros.
   + if_tac; auto.
-    destruct H3 as [p0 ?].
+    destruct H4 as [p0 ?].
     exists p0.
-    rewrite H3; f_equal.
+    rewrite H4; f_equal.
     f_equal.
     extensionality ts; clear ts.
-    clear H3 H4 p0.
+    clear H4 H5 p0.
+    apply ext_level in H3.
     apply predicates_hered.pred_ext; hnf; intros ? [? ?]; split; auto.
     - apply necR_level in H2.
-      rewrite <- H0 by omega; auto.
+      rewrite <- H0 by lia; auto.
     - apply necR_level in H2.
-      rewrite H0 by omega; auto.
+      rewrite H0 by lia; auto.
   + if_tac; auto.
-    destruct H3 as [p0 ?].
+    destruct H4 as [p0 ?].
     exists p0.
-    rewrite H3; f_equal.
+    rewrite H4; f_equal.
     f_equal.
     extensionality ts; clear ts.
-    clear H3 H4 p0.
+    clear H4 H5 p0.
+    apply ext_level in H3.
     apply predicates_hered.pred_ext; hnf; intros ? [? ?]; split; auto.
     - apply necR_level in H2.
-      rewrite H0 by omega; auto.
+      rewrite H0 by lia; auto.
     - apply necR_level in H2.
-      rewrite <- H0 by omega; auto.
+      rewrite <- H0 by lia; auto.
 Qed.
 
 Lemma rec_inv1_nonexpansive: forall sh v Q,
@@ -313,7 +168,7 @@ Proof.
     intros n ?.
     split; intros; hnf; intros; auto.
   }
-  rewrite <- subtypes.eqp_later.
+  eapply predicates_hered.derives_trans, subtypes.eqp_later1.
   eapply predicates_hered.derives_trans, predicates_hered.now_later.
   apply nonexpansive_lock_inv.
 Qed.
@@ -338,24 +193,12 @@ Proof.
   split; intros; hnf; intros; auto.
 Qed.
 
-Lemma exclusive_weak_exclusive: forall R,
-  exclusive_mpred R ->
-  TT |-- weak_exclusive_mpred R.
-Proof.
-  intros.
-  change (predicates_hered.derives TT (weak_exclusive_mpred R)).
-  intros w _.
-  simpl.
-  eapply derives_trans, H.
-  apply sepcon_derives; apply approx_derives.
-Qed.
-
 Lemma rec_inv_weak_rec_inv: forall sh v Q R,
   rec_inv sh v Q R ->
   TT |-- weak_rec_inv sh v Q R.
 Proof.
   intros.
-  change (predicates_hered.derives TT (weak_rec_inv sh v Q R)).
+  constructor.
   intros w _.
   hnf in H |- *.
   intros.
