concurrency/juicy/semax_simlemmas.v
@@ -35,8 +35,8 @@ Require Import VST.veric.seplog.
 Require Import VST.floyd.coqlib3.
 Require Import VST.sepcomp.step_lemmas.
 Require Import VST.sepcomp.event_semantics.
-Require Import VST.concurrency.semax_conc_pred.
-Require Import VST.concurrency.semax_conc.
+Require Import VST.concurrency.juicy.semax_conc_pred.
+Require Import VST.concurrency.juicy.semax_conc.
 Require Import VST.concurrency.common.threadPool.
 Require Import VST.concurrency.juicy.juicy_machine.
 Require Import VST.concurrency.common.HybridMachineSig.
@@ -57,7 +57,6 @@ Require Import VST.veric.Clight_aging_lemmas.
 Import Clight_initial_world.
 Import Clight_seplog.
 Import ghost_PCM.
-Set Bullet Behavior "Strict Subproofs".
 
 Lemma flat_inj_incr : forall b b', (b <= b')%positive ->
   inject_incr (Mem.flat_inj b) (Mem.flat_inj b').
